solutions/compatibility.v
@@ -185,6 +185,23 @@ Section compatibility.
       (iSplitL; [by eauto 12 with iFrame | iExists _, _; eauto]).
   Qed.
 
+  (** ** Recursive types *)
+  (** Hint: A crucial ingredient for these proofs is the lemma [sem_ty_unfold]. *)
+  Lemma Fold_sem_typed Γ e C `{!NonExpansive C} :
+    Γ ⊨ e : C (μ A, C A)%sem_ty -∗ Γ ⊨ (fold: e) : μ A, C A.
+  (* SOLUTION *) Proof.
+    iIntros "#H" (vs) "!# #HΓ /=". wp_pures.
+    wp_apply (wp_wand with "(H [//])"); iIntros (w) "#HC".
+    rewrite /rec_fold. wp_lam. iModIntro. by iApply sem_ty_unfold.
+  Qed.
+  Lemma Unfold_sem_typed Γ e C `{!NonExpansive C} :
+    Γ ⊨ e : (μ A, C A) -∗ Γ ⊨ (unfold: e) : C (μ A, C A)%sem_ty.
+  (* SOLUTION *) Proof.
+    iIntros "#H" (vs) "!# #HΓ /=".
+    wp_apply (wp_wand with "(H [//])"); iIntros (w) "#HC".
+    rewrite sem_ty_unfold. rewrite /rec_unfold. by wp_lam.
+  Qed.
+
   (** ** Operators *)
   Lemma UnOp_sem_typed Γ e op A B :
     SemTyUnOp op A B → Γ ⊨ e : A -∗ Γ ⊨ UnOp op e : B.
